LemmasForClauses.AndClauses.fst
@@ -47,7 +47,8 @@ let and_clauses_in_interval (v1:int) (v2:int) (v:int) (n:nat) (start_interval:na
     = ()
 
 
-let prove_same_value_and (f1:formula_t) (rf1 : list (list int)) (v1:int)
+#set-options "--split_queries always"
+let prove_same_value_can_extend_and (f1:formula_t) (rf1 : list (list int)) (v1:int)
                          (f2:formula_t) (rf2 : list (list int)) (v2:int)
                          (n:nat) (start_interval:nat) (mid:nat) (v:int) (end_interval:nat)
                          (rf : list (list int))
@@ -59,7 +60,8 @@ let prove_same_value_and (f1:formula_t) (rf1 : list (list int)) (v1:int)
                       rf = rf1 @ rf2 @ (and_clauses v1 v2 v) /\
                       end_interval = v + 1)
             (ensures valid (And f1 f2) rf v n start_interval end_interval /\
-                     tseitin_same_value (And f1 f2) rf v n start_interval end_interval)
+                     tseitin_same_value (And f1 f2) rf v n start_interval end_interval /\
+                     tseitin_can_extend (And f1 f2) rf v n start_interval end_interval)
     = LP.append_assoc rf1 rf2 (and_clauses v1 v2 v);
       append_valid_cnf_formulas rf1 rf2;
       append_valid_cnf_formulas (rf1 @ rf2) (and_clauses v1 v2 v);
@@ -74,102 +76,29 @@ let prove_same_value_and (f1:formula_t) (rf1 : list (list int)) (v1:int)
       assert (valid (And f1 f2) rf v n start_interval end_interval);
 
       let aux (tau : list bool) 
-          : Lemma (requires L.length tau >= end_interval /\
-                            variables_up_to_cnf_formula rf (L.length tau) /\
+          : Lemma (requires L.length tau >= end_interval &&
+                            variables_up_to_cnf_formula rf (L.length tau) &&
                             truth_value_cnf_formula rf tau)
                   (ensures variables_up_to (And f1 f2) (L.length tau) &&
                            variables_up_to_literal (pos_var_to_lit v) (L.length tau) &&truth_value_literal (pos_var_to_lit v) tau = truth_value (And f1 f2) tau)
           = assert (variables_up_to_cnf_formula rf (L.length tau));
+
             variables_up_to_monotone f1 n (L.length tau);
             variables_up_to_monotone f2 n (L.length tau);
-            assert (truth_value_literal (pos_var_to_lit v1) tau = truth_value f1 tau);
-            assert (truth_value_literal (pos_var_to_lit v2) tau = truth_value f2 tau);
-            lemma_and_clauses v1 v2 v tau;
-            assert (truth_value_literal (pos_var_to_lit v) tau = truth_value (And f1 f2) tau)
+            assert (variables_up_to_cnf_formula rf1 (L.length tau));
+            assert (variables_up_to_cnf_formula rf2 (L.length tau));
+            assert (variables_up_to_cnf_formula (and_clauses v1 v2 v) (L.length tau));
+           
+            append_valid_cnf_formulas rf2 (and_clauses v1 v2 v);
+            append_variables_in_interval rf2 (and_clauses v1 v2 v) n start_interval end_interval;
+            assert (variables_in_interval (rf2 @ (and_clauses v1 v2 v)) n start_interval end_interval);
+            assert (variables_up_to_cnf_formula (rf2 @ (and_clauses v1 v2 v)) (L.length tau));
+
+            true_parts_of_cnf_formula (rf1 @ rf2) (and_clauses v1 v2 v) tau;
+            true_parts_of_cnf_formula rf1 (rf2 @ (and_clauses v1 v2 v)) tau;
+            true_parts_of_cnf_formula rf1 rf2 tau;
+
+            lemma_and_clauses v1 v2 v tau
       in
       forall_intro (move_requires aux)
-
-
-let prove_can_extend_and (f1:formula_t) (rf1 : list (list int)) (v1:int) 
-                         (f2:formula_t) (rf2 : list (list int)) (v2:int) 
-                         (n:nat) (start_interval:nat) (mid:nat) (v:int) (end_interval:nat)
-                         (rf :list (list int))
-    : Lemma (requires n <= start_interval /\ start_interval <= mid /\ mid <= v /\
-                      valid f1 rf1 v1 n start_interval mid /\
-                      tseitin_can_extend f1 rf1 v1 n start_interval mid /\
-                      valid f2 rf2 v2 n mid v /\
-                      tseitin_can_extend f2 rf2 v2 n mid v /\
-                      rf = rf1 @ rf2 @ (and_clauses v1 v2 v) /\
-                      end_interval = v + 1)
-            (ensures valid (And f1 f2) rf v n start_interval end_interval /\
-                     tseitin_can_extend (And f1 f2) rf v n start_interval end_interval)
-    = LP.append_assoc rf1 rf2 (and_clauses v1 v2 v);
-      append_valid_cnf_formulas rf1 rf2;
-      append_valid_cnf_formulas (rf1 @ rf2) (and_clauses v1 v2 v);
-
-      variables_in_interval_monotone rf1 n start_interval start_interval mid end_interval;
-      variables_in_interval_monotone rf2 n mid start_interval v end_interval;
-
-      and_clauses_in_interval v1 v2 v n start_interval mid end_interval;
-      append_variables_in_interval rf1 rf2 n start_interval end_interval;
-      append_variables_in_interval (rf1 @ rf2) (and_clauses v1 v2 v) n start_interval end_interval;
-      assert (valid (And f1 f2) rf v n start_interval end_interval)
-      
-      // let aux (tau : list bool)
-      //     : Lemma (requires L.length tau = n)
-      //             (ensures L.length tau = n /\
-      //                      can_extend tau (And f1 f2) rf v n start_interval end_interval)
-      //     = let conditions1 (tau1 : list bool) : Tot bool =
-      //           is_prefix tau tau1 &&
-      //           L.length tau1 = mid &&
-      //           truth_value_cnf_formula rf1 tau1 &&
-      //           truth_value f1 tau = truth_value_literal (pos_var_to_lit v1) tau1
-      //       in
-      //       assume (exists x . conditions1 x);
-      //       let tau1 = extract_value conditions1 in
-      //       assert (is_prefix tau tau1);
-      //       assert (L.length tau1 = mid);
-
-
-      //       let conditions2 (tau2 : list bool) : Tot bool =
-      //           is_prefix tau tau2 &&
-      //           L.length tau2 = v &&
-      //           truth_value_cnf_formula rf2 tau2 &&
-      //           truth_value f2 tau = truth_value_literal (pos_var_to_lit v2) tau2
-      //       in
-      //       assume (exists x . conditions2 x);
-      //       let tau2 = extract_value conditions2 in
-      //       assert (is_prefix tau tau2);
-      //       assert (L.length tau2 = v);
-
-
-      //       let tau' = combine tau tau1 tau2 n start_interval mid v (truth_value (And f1 f2) tau) in
-      //       assert (L.length tau' = v + 1);
-
-      //       // assert (interval_of_list tau' 0 n = interval_of_list tau 0 n);
-      //       assert (interval_of_list tau' start_interval mid = interval_of_list tau1 start_interval mid);
-      //       assert (interval_of_list tau' mid v = interval_of_list tau2 mid v);
-      //       assert (L.index tau' v = truth_value (And f1 f2) tau);
-
-      //       assert (truth_value_literal (pos_var_to_lit v) tau' = truth_value (And f1 f2) tau);
-      //       assert (truth_value_literal (neg_var_to_lit v) tau' = not (truth_value (And f1 f2) tau));
-
-      //       is_prefix_then_is_interval tau tau1;
-      //       transfer_truth_value rf1 tau1 tau' n start_interval mid;
-      //       is_prefix_then_is_interval tau tau2;
-      //       transfer_truth_value rf2 tau2 tau' n mid v;
-
-      //       transfer_truth_value_lit (pos_var_to_lit v1) tau1 tau' n start_interval mid;
-      //       // assert (truth_value_literal (pos_var_to_lit v1) tau' = truth_value f1 tau);
-      //       transfer_truth_value_lit (neg_var_to_lit v1) tau1 tau' n start_interval mid;
-      //       // assert (truth_value_literal (neg_var_to_lit v1) tau' = not (truth_value f1 tau));
-            
-      //       transfer_truth_value_lit (pos_var_to_lit v2) tau2 tau' n mid v;
-      //       // assert (truth_value_literal (pos_var_to_lit v2) tau' = truth_value f2 tau);
-      //       transfer_truth_value_lit (neg_var_to_lit v2) tau2 tau' n mid v;
-      //       // assert (truth_value_literal (neg_var_to_lit v2) tau' = not (truth_value f1 tau));
-
-      //       lemma_and_clauses v1 v2 v tau';
-      //       assert (can_extend tau (And f1 f2) rf v n start_interval end_interval)
-      // in
-      // forall_intro (move_requires aux)
+#reset-options
