LemmasForClauses.NotClauses.fst
@@ -3,7 +3,6 @@ module LemmasForClauses.NotClauses
 open FStar.List.Tot
 module L = FStar.List.Tot.Base
 open FStar.Classical
-// open Utils
 open FormulaT
 open CnfFormula
 open TseitinCore
@@ -42,7 +41,8 @@ let not_clauses_in_interval (v1:int) (v:int) (n:nat) (start_interval:nat) (end_i
     = ()
 
 
-let prove_same_value_not (f1:formula_t) (rf1 : list (list int)) (v1:int) (n:nat)
+#set-options "--split_queries always"
+let prove_same_value_can_extend_not (f1:formula_t) (rf1 : list (list int)) (v1:int) (n:nat)
                          (start_interval:nat) (v:int) (end_interval:nat)
                          (rf : list (list int)) 
     : Lemma (requires n <= start_interval /\ start_interval <= v /\
@@ -51,7 +51,8 @@ let prove_same_value_not (f1:formula_t) (rf1 : list (list int)) (v1:int) (n:nat)
                       rf = rf1 @ (not_clauses v1 v) /\
                       end_interval = v + 1)
             (ensures valid (Not f1) rf v n start_interval end_interval /\
-                     tseitin_same_value (Not f1) rf v n start_interval end_interval)
+                     tseitin_same_value (Not f1) rf v n start_interval end_interval /\
+                     tseitin_can_extend (Not f1) rf v n start_interval end_interval)
     = append_valid_cnf_formulas rf1 (not_clauses v1 v);
       variables_in_interval_monotone rf1 n start_interval start_interval v end_interval;
       not_clauses_in_interval v1 v n start_interval end_interval;
@@ -65,53 +66,8 @@ let prove_same_value_not (f1:formula_t) (rf1 : list (list int)) (v1:int) (n:nat)
                            variables_up_to_literal (pos_var_to_lit v) (L.length tau) &&
                            truth_value_literal (pos_var_to_lit v) tau = truth_value (Not f1) tau)
           = variables_up_to_monotone f1 n (L.length tau);
-            assert (truth_value_literal (pos_var_to_lit v1) tau = truth_value f1 tau);
-            lemma_not_clauses v1 v tau;
-            assert (truth_value_literal (pos_var_to_lit v) tau = truth_value (Not f1) tau)
+            true_parts_of_cnf_formula rf1 (not_clauses v1 v) tau;
+            lemma_not_clauses v1 v tau
       in
       forall_intro (move_requires aux)
-
-
-let prove_can_extend_not (f1:formula_t) (rf1 : list (list int)) (v1:int) (n:nat)
-                         (start_interval:nat) (v:int) (end_interval:nat) (rf : list (list int))
-    : Lemma (requires n <= start_interval /\ start_interval <= v /\ v < end_interval /\
-                      valid f1 rf1 v1 n start_interval v /\
-                      tseitin_can_extend f1 rf1 v1 n start_interval v /\
-                      rf = rf1 @ (not_clauses v1 v) /\
-                      end_interval = v + 1)
-            (ensures valid (Not f1) rf v n start_interval end_interval /\
-                     tseitin_can_extend (Not f1) rf v n start_interval end_interval)
-    = append_valid_cnf_formulas rf1 (not_clauses v1 v);
-      variables_in_interval_monotone rf1 n start_interval start_interval v end_interval;
-      not_clauses_in_interval v1 v n start_interval end_interval;
-      append_variables_in_interval rf1 (not_clauses v1 v) n start_interval end_interval;
-      assert (valid (Not f1) rf v n start_interval end_interval)
-
-    //   let aux (tau : list bool) 
-    //       : Lemma (requires L.length tau = n)
-    //               (ensures L.length tau = n /\
-    //                        can_extend tau (Not f1) rf v n start_interval end_interval)
-    //       = assert (can_extend tau f1 rf1 v1 n start_interval v);
-    //         assert (valid_literal (pos_var_to_lit v1));
-            
-    //         let conditions (tau1 : list bool) =
-    //             is_prefix tau tau1 &&
-    //             L.length tau1 = v &&
-    //             truth_value_cnf_formula rf1 tau1 &&
-    //             truth_value f1 tau = truth_value_literal (pos_var_to_lit v1) tau1
-    //         in
-    //         assume (exists x . conditions x);
-    //         let tau1 = extract_value conditions in
-
-    //         negate_literal v1 tau1;
-
-    //         let tau' = combine1 tau tau1 n start_interval v (truth_value (Not f1) tau) in
-    //         is_prefix_then_is_interval tau tau1;
-    //         transfer_truth_value rf1 tau1 tau' n start_interval v
-
-            // transfer_truth_value_lit (pos_var_to_lit v1) tau1 tau' n start_interval v;
-            // transfer_truth_value_lit (neg_var_to_lit v1) tau1 tau' n start_interval v
-
-            //lemma_not_clauses v1 v tau'
-    //   in
-    //   forall_intro (move_requires aux) 
+#reset-options
