Main.fst
@@ -5,7 +5,7 @@ open FStar.String
 open FStar.IO
 open FormulaT
 open Cnf
-// open Tseitin
+open Tseitin
 
 
 
@@ -15,7 +15,13 @@ let rec print_clause (clause : list int) : string
       | hd::tl -> 
            let r = print_clause tl in
            if r = "" then string_of_int hd
-           else concat " \/ " [string_of_int hd; r]
+           else
+           (
+              if hd < 0 then 
+                 let aux = concat "" ["~("; string_of_int (-hd); ")"] in
+                 concat " or " [aux; r]
+              else concat " or " [string_of_int hd; r]
+           )
 
 
 let rec print_cnf_formula (f : list (list int)) : string
@@ -24,7 +30,7 @@ let rec print_cnf_formula (f : list (list int)) : string
       | hd::tl ->
            let r = print_cnf_formula tl in
            if r = "" then concat "" ["("; print_clause hd; ")"]
-           else concat " /\ " [concat "" ["("; print_clause hd; ")"]; r]
+           else concat " and " [concat "" ["("; print_clause hd; ")"]; r]
 
 
 let main = let f0 = Var 0 in
@@ -43,15 +49,13 @@ let main = let f0 = Var 0 in
            let var_for_rule_9 = Not (Not f0) in
            let test_formula = DImplies (Or f1 f2) f0 in
 
-           let out1 = FStar.Printf.sprintf "%s\n" (pretty_print test_formula) in
+           let out1 = FStar.Printf.sprintf "Formula: %s\n\n" (pretty_print test_formula) in
            print_string out1;
 
            let cnf = convert_to_cnf test_formula in
-           let out2 = FStar.Printf.sprintf "%s\n" (pretty_print cnf) in
+           let out2 = FStar.Printf.sprintf "Algoritm clasic:\n%s\n\n" (pretty_print cnf) in
            print_string out2;
 
-        //    let tseitin_f = tseitin test_formula in
-           let tseitin_f = [[1;2;3]; [0;1]; [2;4]] in
-           let out3 = FStar.Printf.sprintf "%s\n" (print_cnf_formula tseitin_f) in
+           let tseitin_f = tseitin test_formula in
+           let out3 = FStar.Printf.sprintf "Tseitin:\n%s\n\n" (print_cnf_formula tseitin_f) in
            print_string out3
-
