TseitinCore.fst
@@ -3,12 +3,17 @@ module TseitinCore
 open FStar.List.Tot
 module L = FStar.List.Tot.Base
 module LP = FStar.List.Tot.Properties
-open FStar.Tactics
-open FStar.Calc
 open Utils
 open FormulaT
 open CnfFormula
 
+
+
+let valid (f:formula_t) (rf : list (list int)) (v:int) (n:nat) (start_interval:nat) (end_interval:nat)
+    = n <= start_interval /\ start_interval <= end_interval /\
+      variables_up_to f n /\ valid_cnf_formula rf /\ valid_variable v /\
+      variable_in_interval v n start_interval end_interval /\
+      variables_in_interval rf n start_interval end_interval
 
 
 let extend (tau : list bool) (tau' : list bool) (n:nat) (start_interval:nat) (end_interval:nat)
@@ -24,19 +29,9 @@ let extend (tau : list bool) (tau' : list bool) (n:nat) (start_interval:nat) (en
       LP.append_assoc tau falses tau';
       LP.append_length tau falses;
       LP.append_length (tau @ falses) tau';
-      assert (L.length r = end_interval);
       same_values_append [] tau (falses @ tau');
-      assert (interval_of_list r 0 n = tau);
       same_values_append (tau @ falses) tau' [];
-      assert (interval_of_list r start_interval end_interval = tau');
       r
-
-
-let valid (f:formula_t) (rf : list (list int)) (v:int) (n:nat) (start_interval:nat) (end_interval:nat)
-    = n <= start_interval /\ start_interval <= end_interval /\
-      variables_up_to f n /\ valid_cnf_formula rf /\ valid_variable v /\
-      variable_in_interval v n start_interval end_interval /\
-      variables_in_interval rf n start_interval end_interval
 
 
 let can_extend (tau : list bool) 
@@ -46,7 +41,7 @@ let can_extend (tau : list bool)
                (n:nat {L.length tau = n}) 
                (start_interval:nat) 
                (end_interval:nat {valid f rf v n start_interval end_interval})
-    = exists (tau' : list bool) . (L.length tau <= L.length tau' && L.length tau' = end_interval) ==> 
+    = exists (tau' : list bool) . (is_prefix tau tau' && L.length tau' = end_interval) ==> 
         (truth_value_cnf_formula rf tau' &&
         truth_value f tau = truth_value_literal (pos_var_to_lit v) tau')
 
@@ -63,294 +58,3 @@ let tseitin_same_value (f:formula_t) (rf : list (list int)) (v:int) (n:nat) (sta
          variables_up_to_monotone f n (L.length tau);
          truth_value_literal (pos_var_to_lit v) tau = truth_value f tau
       )
-
-
-let combine (tau : list bool) (tau1 : list bool) (tau2 : list bool) (n:nat) 
-            (start_interval:nat) (mid:nat) (end_interval:nat) (last:bool)
-    : Pure (list bool) (requires n <= start_interval && start_interval <= mid && mid <= end_interval &&
-                                 L.length tau = n && L.length tau1 = mid && L.length tau2 = end_interval)
-                       (ensures fun r -> (L.length r = end_interval + 1 &&
-                                          interval_of_list r 0 n = tau &&
-                                          interval_of_list r start_interval mid = interval_of_list tau1 start_interval mid &&
-                                          interval_of_list r mid end_interval = interval_of_list tau2 mid end_interval && 
-                                          interval_of_list r end_interval (end_interval + 1) = [last]))
-    = let falses = n_falses (start_interval - n) in
-      let from_tau1 = interval_of_list tau1 start_interval mid in
-      let from_tau2 = interval_of_list tau2 mid end_interval in
-      let l1 = tau @ falses in
-      let l2 = l1 @ from_tau1 in
-      let l3 = l2 @ from_tau2 in
-      let r = l3 @ [last] in
-
-      LP.append_assoc tau falses from_tau1;
-      LP.append_assoc tau falses (from_tau1 @ from_tau2);
-      LP.append_assoc tau falses (from_tau1 @ from_tau2 @ [last]);
-      LP.append_assoc l1 from_tau1 from_tau2;
-      LP.append_assoc l1 from_tau1 (from_tau2 @ [last]);
-      LP.append_assoc l2 from_tau2 [last];
-
-      LP.append_length tau falses;
-      assert (L.length l1 = L.length tau + L.length falses);
-      assert (L.length tau = n);
-      assert (L.length falses = start_interval - n);
-      assert (L.length l1 = start_interval);
-      LP.append_length l1 from_tau1;
-      assert (L.length l2 = L.length l1 + L.length from_tau1);
-      assert (L.length l1 = start_interval);
-      assert (L.length from_tau1 = mid - start_interval);
-      assert (L.length l2 = mid) by compute ();
-      LP.append_length l2 from_tau2;
-      assert (L.length l3 = L.length l2 + L.length from_tau2);
-      assert (L.length l2 = mid);
-      assert (L.length from_tau2 = end_interval - mid);
-      assert (L.length l3 = end_interval) by compute ();
-      LP.append_length l3 [last];
-      assert (L.length r = L.length l3 + L.length [last]);
-      assert (L.length l3 = end_interval);
-      assert (L.length [last] = 1) by compute ();
-      assert (L.length r = end_interval + 1) by compute ();
-      
-
-      assert (r = [] @ tau @ (falses @ from_tau1 @ from_tau2 @ [last]));
-      interval_append_fst tau (falses @ from_tau1 @ from_tau2 @ [last]);
-      assert (interval_of_list r 0 n = tau);
-
-      assert (r = l1 @ from_tau1 @ (from_tau2 @ [last]));
-      same_values_append l1 from_tau1 (from_tau2 @ [last]);
-      assert (interval_of_list r start_interval mid = interval_of_list tau1 start_interval mid);
-
-      assert (r = l2 @ from_tau2 @ [last]);
-      same_values_append l2 from_tau2 [last];
-      assert (interval_of_list r mid end_interval = interval_of_list tau2 mid end_interval);
-
-      assert (r = l3 @ [last] @ []);
-      same_values_append l3 [last] [];
-      assert (interval_of_list r end_interval (end_interval + 1) = [last]);
-
-      r
-
-
-let combine1 (tau : list bool) (tau1 : list bool) 
-             (n:nat) (start_interval:nat) (v:int) (last:bool)
-    : Pure (list bool) (requires n <= start_interval && start_interval <= v &&
-                                 L.length tau = n &&
-                                 L.length tau1 = v)
-                       (ensures fun r -> (L.length r = v + 1 &&
-                                          interval_of_list r 0 n = tau &&
-                                          interval_of_list r start_interval v = interval_of_list tau1 start_interval v &&
-                                          interval_of_list r v (v + 1) = [last]))
-    = let falses = n_falses (start_interval - n) in
-      let from_tau1 = interval_of_list tau1 start_interval v in
-      let l1 = tau @ falses in
-      let l2 = l1 @ from_tau1 in
-      let r = l2 @ [last] in
-
-      LP.append_assoc tau falses from_tau1;
-      LP.append_assoc tau falses (from_tau1 @ [last]);
-      LP.append_assoc l1 from_tau1 [last];
-
-      LP.append_length tau falses;
-      assert (L.length l1 = start_interval) by compute ();
-      LP.append_length l1 from_tau1;
-      assert (L.length l2 = v) by compute ();
-      LP.append_length l2 [last];
-      assert (L.length r = v + 1) by compute ();
-
-      assert (r = [] @ tau @ (falses @ from_tau1 @ [last]));
-      interval_append_fst tau (falses @ from_tau1 @ [last]);
-      assert (interval_of_list r 0 n = tau);
-
-      assert (r = l1 @ from_tau1 @ [last]);
-      same_values_append l1 from_tau1 [last];
-      assert (interval_of_list r start_interval v = interval_of_list tau1 start_interval v);
-
-      assert (r = l2 @ [last] @ []);
-      same_values_append l2 [last] [];
-      assert (interval_of_list r v (v + 1) = [last]);
-      r
-
-
-// let not_clauses (v1:int {valid_variable v1})
-//                 (v:int {valid_variable v})
-//     : r : list (list int) {valid_cnf_formula r}
-//     = [[neg_var_to_lit v; neg_var_to_lit v1];
-//        [pos_var_to_lit v1; pos_var_to_lit v]]
-
-
-// let or_clauses (v1:int {valid_variable v1}) 
-//                (v2:int {valid_variable v2}) 
-//                (v:int {valid_variable v}) 
-//     : r : list (list int) {valid_cnf_formula r}
-//     = [[neg_var_to_lit v; pos_var_to_lit v1; pos_var_to_lit v2];
-//        [neg_var_to_lit v1; pos_var_to_lit v];
-//        [neg_var_to_lit v2; pos_var_to_lit v]]
-
-
-// let and_clauses (v1:int {valid_variable v1}) 
-//                 (v2:int {valid_variable v2}) 
-//                 (v:int {valid_variable v}) 
-//     : r : list (list int) {valid_cnf_formula r}
-//     = [[neg_var_to_lit v; pos_var_to_lit v1];
-//        [neg_var_to_lit v; pos_var_to_lit v2];
-//        [neg_var_to_lit v1; neg_var_to_lit v2; pos_var_to_lit v]]
-
-
-// let implies_clauses (v1:int {valid_variable v1}) 
-//                     (v2:int {valid_variable v2}) 
-//                     (v:int {valid_variable v}) 
-//     : r : list (list int) {valid_cnf_formula r}
-//     = [[neg_var_to_lit v; neg_var_to_lit v1; pos_var_to_lit v2];
-//        [pos_var_to_lit v1; pos_var_to_lit v];
-//        [neg_var_to_lit v2; pos_var_to_lit v]]
-
-
-// let dimplies_clauses (v1:int {valid_variable v1}) 
-//                      (v2:int {valid_variable v2}) 
-//                      (v:int {valid_variable v}) 
-//     : r : list (list int) {valid_cnf_formula r /\ L.length r = 4 /\
-//                            r = [L.index r 0; L.index r 1; L.index r 2; L.index r 3] /\
-//                            L.index r 0 = [neg_var_to_lit v; neg_var_to_lit v1; pos_var_to_lit v2] /\ L.length (L.index r 0) = 3 /\
-//                            L.index r 1 = [neg_var_to_lit v1; neg_var_to_lit v2; pos_var_to_lit v] /\ L.length (L.index r 1) = 3 /\
-//                            L.index r 2 = [pos_var_to_lit v1; pos_var_to_lit v2; pos_var_to_lit v] /\ L.length (L.index r 2) = 3 /\
-//                            L.index r 3 = [neg_var_to_lit v; neg_var_to_lit v2; pos_var_to_lit v1] /\ L.length (L.index r 3) = 3}
-//     = [[neg_var_to_lit v; neg_var_to_lit v1; pos_var_to_lit v2];
-//        [neg_var_to_lit v1; neg_var_to_lit v2; pos_var_to_lit v];
-//        [pos_var_to_lit v1; pos_var_to_lit v2; pos_var_to_lit v];
-//        [neg_var_to_lit v; neg_var_to_lit v2; pos_var_to_lit v1]]
-
-
-// let not_clauses_up_to (v1:int) (v:int) (n:nat)
-//     : Lemma (requires valid_variable v1 && valid_variable v &&
-//                       n > v1 && n > v)
-//             (ensures variables_up_to_cnf_formula (not_clauses v1 v) n)
-//     = ()
-
-
-// let lemma_not_clauses (v1:int) (v:int) (tau : list bool)
-//     : Lemma (requires valid_variable v1 && valid_variable v && L.length tau > v && L.length tau > v1)
-//             (ensures variables_up_to_cnf_formula (not_clauses v1 v) (L.length tau) /\
-//                      truth_value_cnf_formula (not_clauses v1 v) tau <==> 
-//                        ((not (truth_value_literal (pos_var_to_lit v1) tau)) <==> 
-//                        truth_value_literal (pos_var_to_lit v) tau))
-//     = not_clauses_up_to v1 v (L.length tau)
-
-
-// let or_clauses_up_to (v1:int) (v2:int) (v:int) (n:nat)
-//     : Lemma (requires valid_variable v1 && valid_variable v2 && valid_variable v &&
-//                       n > v1 && n > v2 && n > v)
-//             (ensures variables_up_to_cnf_formula (or_clauses v1 v2 v) n)
-//     = ()
-
-
-// let lemma_or_clauses (v1:int) (v2:int) (v:int) (tau : list bool)
-//     : Lemma (requires valid_variable v1 && valid_variable v2 && valid_variable v &&
-//                       L.length tau > v1 && L.length tau > v2 && L.length tau > v)
-//             (ensures variables_up_to_cnf_formula (or_clauses v1 v2 v) (L.length tau) /\
-//                      truth_value_cnf_formula (or_clauses v1 v2 v) tau <==>
-//                         ((truth_value_literal (pos_var_to_lit v1) tau || 
-//                         truth_value_literal (pos_var_to_lit v2) tau) <==>
-//                         truth_value_literal (pos_var_to_lit v) tau))
-//     = or_clauses_up_to v1 v2 v (L.length tau)
-
-
-// let and_clauses_up_to (v1:int) (v2:int) (v:int) (n:nat)
-//     : Lemma (requires valid_variable v1 && valid_variable v2 && valid_variable v &&
-//                       n > v1 && n > v2 && n > v)
-//             (ensures variables_up_to_cnf_formula (and_clauses v1 v2 v) n)
-//     = ()
-
-
-// let lemma_and_clauses (v1:int) (v2:int) (v:int) (tau : list bool)
-//     : Lemma (requires valid_variable v1 && valid_variable v2 && valid_variable v &&
-//                       L.length tau > v1 && L.length tau > v2 && L.length tau > v)
-//             (ensures variables_up_to_cnf_formula (and_clauses v1 v2 v) (L.length tau) /\
-//                      truth_value_cnf_formula (and_clauses v1 v2 v) tau <==>
-//                         ((truth_value_literal (pos_var_to_lit v1) tau && 
-//                         truth_value_literal (pos_var_to_lit v2) tau) <==>
-//                         truth_value_literal (pos_var_to_lit v) tau))
-//     = and_clauses_up_to v1 v2 v (L.length tau)
-
-
-// let implies_clauses_up_to (v1:int) (v2:int) (v:int) (n:nat)
-//     : Lemma (requires valid_variable v1 && valid_variable v2 && valid_variable v &&
-//                       n > v1 && n > v2 && n > v)
-//             (ensures variables_up_to_cnf_formula (implies_clauses v1 v2 v) n)
-//     = ()
-
-   
-// let lemma_implies_clauses (v1:int) (v2:int) (v:int) (tau : list bool)
-//     : Lemma (requires valid_variable v1 && valid_variable v2 && valid_variable v &&
-//                       L.length tau > v1 && L.length tau > v2 && L.length tau > v)
-//             (ensures variables_up_to_cnf_formula (implies_clauses v1 v2 v) (L.length tau) /\
-//                      truth_value_cnf_formula (implies_clauses v1 v2 v) tau <==>
-//                         ((truth_value_literal (pos_var_to_lit v1) tau ==> 
-//                         truth_value_literal (pos_var_to_lit v2) tau) <==>
-//                         truth_value_literal (pos_var_to_lit v) tau))
-//     = implies_clauses_up_to v1 v2 v (L.length tau)
-
-
-// let dimplies_clauses_aux (v1:int {valid_variable v1}) 
-//                      (v2:int {valid_variable v2}) 
-//                      (v:int {valid_variable v}) 
-//     : r : list (list int) {valid_cnf_formula r /\ L.length r = 4}
-//     = [[neg_var_to_lit v; neg_var_to_lit v1; pos_var_to_lit v2];
-//        [neg_var_to_lit v1; neg_var_to_lit v2; pos_var_to_lit v];
-//        [pos_var_to_lit v1; pos_var_to_lit v2; pos_var_to_lit v];
-//        [neg_var_to_lit v; neg_var_to_lit v2; pos_var_to_lit v1]]
-
-
-// let dimplies_clauses_up_to (v1:int) (v2:int) (v:int) (n:nat)
-//     : Lemma (requires valid_variable v1 && valid_variable v2 && valid_variable v &&
-//                       n > v1 && n > v2 && n > v)
-//             (ensures variables_up_to_cnf_formula (dimplies_clauses_aux v1 v2 v) n /\
-//                      L.mem (L.index (dimplies_clauses_aux v1 v2 v) 2) (dimplies_clauses_aux v1 v2 v) /\
-//                      L.mem (L.index (dimplies_clauses_aux v1 v2 v) 3) (dimplies_clauses_aux v1 v2 v))
-//     = ()
-
-
-// let lemma_dimplies_clauses (v1:int) (v2:int) (v:int) (tau : list bool)
-//     : Lemma (requires valid_variable v1 && valid_variable v2 && valid_variable v &&
-//                       L.length tau > v1 && L.length tau > v2 && L.length tau > v)
-//             (ensures True)
-//             // (ensures variables_up_to_cnf_formula (dimplies_clauses v1 v2 v) (L.length tau) /\
-//             //          truth_value_cnf_formula (dimplies_clauses v1 v2 v) tau <==>
-//             //             ((truth_value_literal (pos_var_to_lit v1) tau <==> 
-//             //             truth_value_literal (pos_var_to_lit v2) tau) <==>
-//             //             truth_value_literal (pos_var_to_lit v) tau))
-//     = let rf = dimplies_clauses v1 v2 v in
-//       dimplies_clauses_up_to v1 v2 v (L.length tau);
-//       assert (forall clause . L.mem clause rf ==> (variables_up_to_clause clause (L.length tau)));
-//       assert (rf = [L.index rf 0; L.index rf 1; L.index rf 2; L.index rf 3]);
-//       assert (truth_value_cnf_formula rf tau <==>
-//                 truth_value_clause (L.index rf 0) tau &&
-//                 truth_value_clause (L.index rf 1) tau &&
-//                 truth_value_clause (L.index rf 2) tau &&
-//                 truth_value_clause (L.index rf 3) tau) by compute ();
-//       assert (L.index rf 0 = [neg_var_to_lit v; neg_var_to_lit v1; pos_var_to_lit v2]);
-//       assert (L.length (L.index rf 0) = 3);
-//       assert (L.index (L.index rf 0) 2 = pos_var_to_lit v2) by compute ();
-//       assert (truth_value_clause (L.index rf 0) tau <==>
-//                 truth_value_literal (L.index (L.index rf 0) 0) tau ||
-//                 truth_value_literal (L.index (L.index rf 0) 1) tau ||
-//                 truth_value_literal (L.index (L.index rf 0) 2) tau) by compute ();
-//       assert (L.index rf 1 = [neg_var_to_lit v1; neg_var_to_lit v2; pos_var_to_lit v]);
-//       assert (L.length (L.index rf 1) = 3);
-//       assert (L.index (L.index rf 1) 2 = pos_var_to_lit v) by compute ();
-//       assert (truth_value_clause (L.index rf 1) tau <==>
-//                 truth_value_literal (L.index (L.index rf 1) 0) tau ||
-//                 truth_value_literal (L.index (L.index rf 1) 1) tau ||
-//                 truth_value_literal (L.index (L.index rf 1) 2) tau) by compute ();
-//       assert (L.index rf 2 = [pos_var_to_lit v1; pos_var_to_lit v2; pos_var_to_lit v]);
-//       assert (L.length (L.index rf 2) = 3);
-//       assert (L.index (L.index rf 2) 2 = pos_var_to_lit v) by compute ();
-//       assert (truth_value_clause (L.index rf 2) tau <==>
-//                 truth_value_literal (L.index (L.index rf 2) 0) tau ||
-//                 truth_value_literal (L.index (L.index rf 2) 1) tau ||
-//                 truth_value_literal (L.index (L.index rf 2) 2) tau) by compute ();
-//       assert (L.index rf 3 = [neg_var_to_lit v; neg_var_to_lit v2; pos_var_to_lit v1]);
-//       assert (L.length (L.index rf 3) = 3);
-//       assert (L.index (L.index rf 3) 2 = pos_var_to_lit v1) by compute ();
-//       assert (truth_value_clause (L.index rf 3) tau <==>
-//                 truth_value_literal (L.index (L.index rf 3) 0) tau ||
-//                 truth_value_literal (L.index (L.index rf 3) 1) tau ||
-//                 truth_value_literal (L.index (L.index rf 3) 2) tau) by compute ()
