Makefile
@@ -27,8 +27,7 @@ all:
 include .depend
 
 $(CACHE_DIR)/%.checked: | .depend
-	$(FSTAR) $< $(ENABLE_HINTS) --hint_file $(HINT_DIR)/$(notdir $<).hints && \
-	touch $@
+	$(FSTAR) $< $(ENABLE_HINTS) && touch $@
 
 # 2. Compile all .ml files to .cmx and link them to get an executable
 $(OUT_DIR):
